\documentclass{article}

\usepackage{amsmath,amssymb}
\usepackage{fullpage}
\usepackage{enumerate}
\usepackage{hyperref}
\usepackage{graphicx}
\graphicspath{{../logos/}}


\begin{document}

\setlength{\tabcolsep}{6pt}
\begin{center} \begin{tabular}{cccc}
	\includegraphics[height=56pt]{SAMF_logo.jpg} &
	\includegraphics[height=56pt]{SAICA_logo.jpg} &
	\includegraphics[height=56pt]{OM_Logo_Stacked_Vignette_on_White_RGB.jpg} &
	\includegraphics[height=56pt]{SAMO2019.png}
\end{tabular} \end{center}


\bigskip


\begin{center}
	\textbf{\Large <LEVEL> Monthly Problem Set Solutions}
\end{center}

\begin{enumerate}

\medskip
\item[1.] % Problem source
Problem statement


\medskip
\item[2.]

\medskip
\item[3.] % Liam
Let $M$ be a positive integer, and let $S$ denote the set of finite sequences of positive integers less than or equal to $M$, including the empty sequence of length zero, which we denote as $\mathbf{0}$.
Also, for a sequence $\mathbf{x} = (x_1, x_2, \dotsc, x_n)$ let $\overline{\mathbf{x}}$ denote the reverse sequence $\overline{\mathbf{x}} = (x_n, x_{n-1}, \dotsc, x_1)$.

Define a function $d$ from $S$ to the integers as follows:
\begin{itemize}
\item $d(\mathbf{0}) = 0$.
\item If $\mathbf{x} = (x_1, x_2, \dotsc, x_n)$ is a sequence of positive length, let $m$ be the largest integer such that $x_1 +x_2 +\dotsb +x_m \leq M$, and let $\mathbf{x}'$ denote the rest of the sequence: $\mathbf{x}' = (x_{m+1}, \dotsc, x_n)$.
Then $d(\mathbf{x}) = 1 +d(\mathbf{x}')$.
\end{itemize}
Show that $d(\mathbf{x}) = d(\overline{\mathbf{x}})$.

\medskip
\item[SOLUTION]
Note that $d$ partitions the sequence $\mathbf{x}$ into sub-sequences $s.t.$ the sum of each sub-sequence does not exceed $M$ and then counts the total amount of these sub-sequences. Let ${s_1, s_2, .., s_{d(\mathbf{x})}}$ be the indices of the  starts of these sub-sequences.

For the partitioning of $\bar{\mathbf{x}}$ we conjecture that none of the sub-sequences can have more than one of these $x_{s_i}$

If there are exist a sub-sequence with at least two of these $s_i$ we have:
\begin{center}
    $M \geq (\sum_{j=s_{i+1}}^{s_i} x_j) = (\sum_{j=s_i}^{s_{i+1}-1} x_j) + x_{s_{i+1}} > M$ 
\end{center}
which is a contradiction $\implies$ each $s_i$ in its own sub-sequence which implies $d(\overline{\mathbf{x}}) \geq d(\mathbf{x})$

Hence $d(\mathbf{x}) = d(\overline{\overline{\mathbf{x}}}) \geq d(\overline{\mathbf{x}}) \geq d(\mathbf{x})\implies d(x) = d(\bar x)$


\medskip
\item[4.]


\medskip
\item[5.]


\medskip
\item[6.]


\medskip
\item[7.]


\medskip
\item[8.]


\end{enumerate}

\end{document}
